theories/lambdaFacts.v
@@ -1,0 +1,96 @@
+Require Import String.
+Require Import -(coercions) qterm.
+
+(*
+This file will have proofs of various facts that I need about lambda calculus to make the
+unification tactic work.
+These will start as Axioms, and I will prove them eventually.
+
+For now, I will focus on the minimal things that I need to make things work, and I'll add
+as needed.
+ *)
+
+Ltac compute_subst H := repeat (try rewrite subst_app in H;
+                          try (rewrite subst_lam in H; simpl in H) ;
+                          try (rewrite subst_var in H; simpl in H;
+                               repeat (rewrite lift_lam, lift_app, lift_var in H))).
+Ltac normalize H := repeat (rewrite beta in H; compute_subst H).
+
+
+
+Inductive PseudoNeutral : QTerm -> Prop :=
+| neu_var : forall {n i}, PseudoNeutral (var n i)
+| neu_const : forall {s}, PseudoNeutral (const s)
+| neu_app : forall {t1 t2}, PseudoNeutral t1 -> PseudoNeutral (app t1 t2).
+
+Theorem lamInj : forall t1 t2 s, <fun `s => `t1> = <fun `s => `t2> -> t1 = t2.
+Proof.
+  intros.
+  pose (var s 0) as x.
+  assert (<(fun `s => `t1) `x> = <(fun `s => `t2) `x>).
+  rewrite H.
+  reflexivity.
+  unfold x in H0.
+  repeat rewrite beta in H0.
+  repeat rewrite subst_id in H0.
+  assumption.
+Qed.
+
+(*Theorem varInj : forall s1 s2 i j, var s1 i = var s2 j -> s1 = s2 /\ i = j.*)
+Theorem varInj : forall s1 s2, var s1 0 = var s2 0 -> s1 = s2.
+Proof.
+  intros.
+  (*
+    Need to use decidable equality on nat and string (or just LEM), and prove by contradiction
+    using consistency.
+   *)
+
+  destruct (String.string_dec s1 s2).
+  assumption.
+  (* The notation is confusing. H is saying that the variables that looks like s1 and s2 are equal.*)
+  pose consistency as c.
+  destruct c as [t1 c].
+  destruct c as [t2 p].
+  pose (var s1 0) as x1.
+  pose (var s2 0) as x2.
+  assert (<(fun `s1 => fun `s2 => `x1) `t1 `t2> = <(fun `s1 => fun `s2 => `x2) `t1 `t2>) as eq.
+  unfold x1, x2.
+  rewrite H.
+  reflexivity.
+  unfold x1, x2 in eq.
+  normalize eq.
+  assert ((eqb s2 s1) = false).
+  {
+    pose (eqb_spec s2 s1) as fact.
+    destruct fact.
+    exfalso.
+    apply n.
+    apply eq_sym.
+    apply e.
+    reflexivity.
+  }.
+  rewrite H0 in eq.
+  simpl in eq.
+  assert (forall s, (eqb s s) = true).
+  {
+    intro s.
+    pose (eqb_spec s s) as fact.
+    destruct fact.
+    reflexivity.
+  exfalso.
+  apply n0.
+  reflexivity.
+  }.
+  rewrite H1 in eq.
+  simpl in eq.
+  normalize eq.
+  rewrite H1 in eq.
+  simpl in eq.
+
+  (*
+    The fact that this doesn't work shows that there is a problem with my substitution rules.
+    The t1 that we get should have been lifted by s2,
+    and then the subst and lift should have cancleded out.
+    This should work.
+   *)
+ 
