theories/lambdaSolve.v
@@ -1,13 +1,30 @@
 Require Import String.
 Require Import qterm.
+Require Import lambdaFacts.
 
-Ltac normalize := repeat (rewrite ?beta; repeat (rewrite ?subst_app) ;
-                          repeat (rewrite ?subst_lam ; simpl) ;
-                          repeat (rewrite ?subst_var ; simpl) ;
-                          repeat (rewrite ?lift_lam, ?lift_app, lift_var)).
+
+
+Ltac compute_subst := repeat (try rewrite subst_app ;
+                          try (rewrite subst_lam ; simpl) ;
+                          try (rewrite subst_var ; simpl;
+                               repeat (rewrite lift_lam, lift_app, lift_var))).
+(* Is there a way to not have this be repetetive with the above? *)
+Ltac compute_subst_in H := repeat (try rewrite subst_app ;
+                          try (rewrite subst_lam in H ; simpl) ;
+                          try (rewrite subst_var in H; simpl;
+                                  repeat (rewrite lift_lam, lift_app, lift_var in H))).
+Ltac normalize := repeat (rewrite beta; compute_subst).
 
 (*
-[ ] - add pairs and stuff to qterm
+[x] - add pairs and stuff to qterm
 [ ] - find old file that had most advanced unification tactic
 [ ] - port to this version
 *)
+
+Ltac proveNeutral := constructor ; repeat constructor.
+
+Ltac lambda_solve :=
+  repeat (
+      match goal with
+      | H : 
+
