theories/testFile.v
@@ -1,0 +1,70 @@
+Require Import String.
+Require Import qterm.
+
+Ltac normalize := repeat (rewrite beta; repeat (repeat (rewrite subst_app) ;
+                          repeat (rewrite subst_lam ; simpl) ;
+                          repeat (rewrite subst_var ; simpl;
+                                  repeat (rewrite lift_lam, lift_app, lift_var)))
+                          ).
+
+Compute <fun x => fun y => x y>.
+
+Definition t1 := <fun x => x>.
+Definition t2 := <fun y => `t1 y>.
+Compute t2.
+
+Theorem example : <(fun x => x) (fun x => x)> = <fun x => x>.
+Proof.
+  normalize.
+  reflexivity.
+Qed.
+
+
+
+
+
+
+
+
+
+
+
+
+
+
+
+
+
+
+
+
+
+
+
+
+
+
+Definition IsA (t : QTerm) : Prop := t = <a>.
+
+Definition IsB (t : QTerm) : Prop := t = <b>.
+
+Definition Arrow (A : QTerm -> Prop) (B : QTerm -> Prop) (t : QTerm) : Prop :=
+  forall (x : QTerm), A x -> B <`t `x>.
+
+Theorem typing_example : Arrow IsA IsB <fun x => b>.
+Proof.
+  unfold Arrow, IsA, IsB.
+  intros.
+  normalize5.
+  reflexivity.
+Qed.
+
+Definition SameArrow T := Arrow T T.
+
+Compute <Pi A (fun a => B)>.
+
+Inductive Well_Typed : QTerm -> QTerm -> QTerm -> Prop:=
+| app : forall t1 t2 A B ctx, Well_Typed ctx <Pi `A `B> t1 -> Well_Typed ctx A t2
+                        -> Well_Typed ctx B <`t1 `t2>.
+
+
